sme/Sme/ITree/WBisim.lean
@@ -1,0 +1,289 @@
+import CoinductivePredicates
+import Sme.ITree.Defs
+import Sme.ITree.Combinators
+
+namespace Sme.ITree
+
+universe u v
+
+variable {E : Type u → Type u} {A B C : Type (u + 1)}
+
+inductive Step : Base E (ITree E A) A → Base E (ITree E A) A → Type _
+  | tau {a b} : Step a.dest b → Step (.tau a) b
+  | ret {v} : Step (.ret v) (.ret v)
+  | vis {e k} : Step (.vis e k) (.vis e k)
+
+namespace Step
+
+theorem eq {a b c : Base E (ITree E A) A}
+    : Step a b → Step a c → b = c
+  | .tau a, .tau b => eq a b
+  | .ret, .ret | .vis, .vis => rfl
+
+instance {X Y : Base E _ A} : Subsingleton (Step X Y) where
+  allEq := ae
+where ae {X Y} : ∀ (a b : Step X Y), a = b
+  | .tau u, .tau v => ae u v ▸ rfl
+  | .ret , .ret | .vis , .vis => rfl
+
+theorem tau_rhs {V : Base E _ A} {v'} : Step V (.tau v') → False
+  | .tau v => tau_rhs v
+
+theorem not_spin {V} (v : Step (spin : ITree E A).dest V) : False := by
+  generalize h : spin.dest = x at v
+  rw [spin.dest_eq] at h
+  induction v
+  case tau ih =>
+    rw [Base.tau.injEq] at h
+    subst h
+    simp only [spin.dest_eq, imp_false, not_true_eq_false] at ih
+  · contradiction
+  · contradiction
+
+theorem not_spin' {V} : Step (.tau (spin : ITree E A)) V → False
+  | .tau a => not_spin a
+
+theorem not_step {V : ITree E A} (v : ∀ {v}, Step V.dest v → False) : V = spin :=
+  bisim ⟨
+    (fun a b => (∀ {x}, Step a x → False) ∧ (∀ {y}, Step b y → False)),
+    fun {a b} ⟨ha, hb⟩ => match a, b with
+      | .ret _,   _        => (ha .ret).elim
+      | .vis _ _, _        => (ha .vis).elim
+      | _,        .ret _   => (hb .ret).elim
+      | _,        .vis _ _ => (hb .vis).elim
+      | .tau _,   .tau _   => .tau ⟨fun h => ha (.tau h), fun h => hb (.tau h)⟩
+      ,
+    ⟨v, not_spin⟩,
+  ⟩
+
+theorem not_step' {V : Base E _ A} (v : ∀ {v}, Step V v → False) : V = (.tau spin) := by
+  refine mk_eq ?_
+  rw [←spin.dest_eq, dest_mk]
+  apply not_step
+  intro _ a
+  rw [mk_dest] at a
+  apply v a
+
+theorem no_middle (V : Base E _ A)
+    : V = .tau spin
+    ∨ (∃ v, Nonempty (Step V (.ret v))) ∨
+    (∃ A e f, Nonempty (Step V (.vis (e : E A) f))) := by 
+  by_cases h : (∀ {v}, Step V v → False)
+  · exact .inl (not_step' h)
+  simp only [not_forall, not_false_eq_true, exists_const_iff, and_true] at h
+  rcases h with ⟨(_|_|_), ⟨p⟩⟩
+  · exact (tau_rhs p).elim
+  · exact .inr <| .inl ⟨_, ⟨p⟩⟩
+  · exact .inr <| .inr ⟨_,_,_, ⟨p⟩⟩
+
+end Step
+
+inductive EStep : Base E (ITree E A) A → Base E (ITree E A) A → Type _
+  | tau {a b} : EStep a.dest b → EStep (.tau a) b
+  | refl a : EStep a a
+
+namespace EStep
+
+def trans : {a b c : Base E (ITree E A) A}
+    → EStep a b → EStep b c → EStep a c
+  | _,_,_, .refl _, .refl _ => .refl _
+  | _,_,_, .refl _, .tau h
+  | _,_,_, .tau h , .refl _ => .tau h
+  | _,_,_, .tau a, .tau b => .tau <| trans a (.tau b)
+
+def step_comp {a b c : Base E _ A} : EStep a b → Step b c → Step a c
+  | .refl _, v => v
+  | .tau h, ha => .tau (step_comp h ha)
+
+theorem spin {a} (h : EStep a ((spin : ITree E A).dest)) : a = spin.dest := by
+  generalize h' : ITree.dest ITree.spin = v at h
+  induction h
+  case tau h =>
+    subst h'
+    specialize h rfl
+    obtain rfl := dest.inj_eq.mp h
+    simp
+  · rfl
+
+end EStep
+
+coinductive WBisim' (E : Type u → Type u) (A : Type (u + 1))
+    : Base E (ITree E A) A → Base E (ITree E A) A → Prop where
+  -- This case only exists for refl spin spin,
+  -- in fact it could be this,
+  -- but that would be harder to prove things about
+  | refl {a} : WBisim' E A a a
+  | ret {a b v}
+      : Step a (.ret v) → Step b (.ret v) → WBisim' E A a b
+  | vis {V e a b a' b'}
+      : Step a (.vis e a') → Step b (.vis e b') →
+        (∀ v : V, WBisim' (a' v).dest (b' v).dest) → WBisim' E A a b
+
+namespace WBisim'
+
+theorem unfold : Is E A (WBisim' E A) :=
+  fun ⟨r, ris, rab⟩ =>
+    match ris rab with
+    | .refl => .refl
+    | .ret a b => .ret a b
+    | .vis a b h => .vis a b fun v => ⟨r, ris, h v⟩
+
+@[refl]
+theorem refl {a} : WBisim' E A a a := ⟨(· = ·), fun v => v ▸ .refl, rfl⟩
+
+theorem ret {a b v} (ha : Step a (.ret v)) (hb : Step b (.ret v))
+    : WBisim' E A a b := ⟨
+  (Nonempty <| Step · (.ret v) × Step · (.ret v)),
+  fun ⟨a, b⟩ => .ret a b,
+  ⟨ha, hb⟩
+⟩
+
+theorem vis {V e a b a' b'}
+      (ha : Step a (.vis e a')) (hb : Step b (.vis e b'))
+      (h : ∀ v : V, WBisim' E A (a' v).dest (b' v).dest)
+      : WBisim' E A a b := ⟨
+  (fun a b => WBisim' E A a b ∨ Nonempty (Step a (.vis e a') × Step b (.vis e b'))),
+  fun
+    | .inl v =>
+      match v.unfold with
+      | .refl => .refl
+      | .ret a b => .ret a b
+      | .vis a b h => .vis a b fun _ => .inl <| h _
+    | .inr ⟨a, b⟩ => .vis a b fun _ => .inl <| h _,
+  .inr ⟨ha, hb⟩
+⟩
+
+@[elab_as_elim]
+theorem cases {a b} {motive : Base E _ A → Base E _ A → Prop}
+    (h : WBisim' E A a b)
+    (hRefl : motive (.tau spin) (.tau spin))
+    (hRet : {v : _} → Step a (.ret v) → Step b (.ret v) → motive a b)
+    (hVis : {V e f g : _}
+      → Step a (.vis e f)
+      → Step b (.vis e g)
+      → (∀ v : V, WBisim' E A (f v).dest (g v).dest) → motive a b)
+    : motive a b :=
+  match h.unfold with
+  | .refl => by
+    rcases Step.no_middle a with (rfl|⟨_, ⟨p⟩⟩|⟨_,_,f,⟨p⟩⟩)
+    · exact hRefl
+    · exact hRet p p
+    · apply hVis p p fun _ => .refl
+  | .ret a b => hRet a b
+  | .vis a b h => hVis a b h
+
+theorem symm {a b} : WBisim' E A a b → WBisim' E A b a :=
+  fun ⟨r, ris, rab⟩ => ⟨
+    fun a b => r b a,
+    fun rab =>
+      match ris rab with
+      | .ret a b => .ret b a
+      | .refl => .refl
+      | .vis a b h => .vis b a h,
+    rab,
+  ⟩
+
+theorem trans {a b c} : WBisim' E A a b → WBisim' E A b c → WBisim' E A a c :=
+  fun ⟨r, ris, rab⟩ ⟨r', ris', rbc⟩ => ⟨
+    (fun a c => r a c ∨ r' a c ∨ ∃ b, r a b ∧ r' b c),
+    fun
+      | .inl v  => (match ris v with
+        | .refl => .refl
+        | .ret a b => .ret a b
+        | .vis a b h => .vis a b fun v => .inl (h v))
+      | .inr <| .inl v  => (match ris' v with
+        | .refl => .refl
+        | .ret a b => .ret a b
+        | .vis a b h => .vis a b fun v => .inr <| .inl (h v))
+      | .inr <| .inr ⟨_, rab, rbc⟩ => (match ris rab, ris' rbc with
+        | .refl, .refl => .refl
+        | .ret a b, .refl
+        | .refl, .ret a b => .ret a b
+        | .vis a b h, .refl => .vis a b (fun x => .inl <| h x)
+        | .refl, .vis a b h => .vis a b (fun x => .inr <| .inl <| h x)
+        | .vis a b h, .vis b' a' h' => by
+          obtain ⟨rfl, rfl, rfl⟩ := (Base.vis.injEq _ _ _ _ _).mp <| b.eq b'
+          exact .vis a a' (fun v => .inr <| .inr <| ⟨_, h v, h' v⟩)
+        | .ret a b, .ret b' a' => by
+          obtain ⟨rfl, rfl, rfl⟩ := (Base.ret.injEq _ _).mp <| b.eq b'
+          exact .ret a a'
+        | .ret _ h, .vis h' _ _
+        | .vis _ h' _, .ret h _ => by
+          have := Step.eq h h'
+          contradiction),
+    .inr <| .inr ⟨_, rab, rbc⟩,
+  ⟩
+
+theorem eqSpin {a} (h : WBisim' E A a spin.dest) : a = spin.dest :=
+  h.cases rfl (fun _ h => (Step.not_spin h).elim) (fun _ h => (Step.not_spin h).elim)
+
+theorem eqSpin' {a} (h : WBisim' E A a (.tau spin)) : a = (.tau spin) :=
+  h.cases rfl (fun _ h => (Step.not_spin' h).elim) (fun _ h => (Step.not_spin' h).elim)
+
+theorem tau {a} : WBisim' E A (Base.tau a) a.dest := ⟨
+  (fun a b => Nonempty (EStep a b)),
+  fun {a b} ⟨ha⟩ => by
+    rcases Step.no_middle b with (rfl|⟨_, ⟨h⟩⟩|⟨_,_,_, ⟨h⟩⟩)
+    · rw [←spin.dest_eq] at ha
+      obtain rfl := ha.spin
+      rw [spin.dest_eq]
+      exact .refl
+    · refine .ret ?_ h
+      exact ha.step_comp h
+    · refine .vis (ha.step_comp h) h fun _ => ⟨.refl _⟩
+  ,
+  ⟨.tau <| .refl _⟩
+⟩
+
+theorem ofEStep {a b} : EStep a b → WBisim' E A a b 
+  | .tau h => .trans tau (ofEStep h)
+  | .refl _ => .refl
+
+end WBisim'
+
+def WBisim {E : Type u → Type u} {A : Type (u + 1)} (a b : ITree E A) : Prop :=
+  WBisim' E A a.dest b.dest
+
+infix:100 " ≈ " => WBisim
+
+namespace WBisim
+
+variable {a b c : ITree E A}
+
+@[refl] theorem refl :   a ≈ a := WBisim'.refl
+@[symm] theorem symm :   a ≈ b → b ≈ a := WBisim'.symm
+@[trans] theorem trans : a ≈ b → b ≈ c → a ≈ c := WBisim'.trans
+
+instance : Equivalence (· ≈ · : ITree E A → _ → _) where
+  refl _ := refl
+  symm := symm
+  trans := trans
+
+theorem eqSpin (h : a ≈ spin) : a = spin :=
+  dest.inj_eq.mp <| WBisim'.eqSpin h
+
+-- TODO:
+@[elab_as_elim]
+theorem cases {motive : ITree E A → ITree E A → Prop}
+    (h : WBisim a b)
+    (hRefl : motive (.tau spin) (.tau spin))
+    (hRet : {v : _} → Step a.dest (.ret v) → Step b.dest (.ret v) → motive a b)
+    (hVis : {V e f g : _}
+      → Step a.dest (.vis e f)
+      → Step b.dest (.vis e g)
+      → (∀ v : V, WBisim (f v) (g v)) → motive a b)
+    : motive a b := by
+  sorry
+
+theorem tau : .tau a ≈ a := by
+  rw [WBisim, dest_tau]
+  exact WBisim'.tau
+
+@[simp]
+theorem tau_bind {f : _ → ITree E B} {a : ITree E A} : bind (.tau a) f ≈ bind a f :=
+  ITree.tau_bind ▸ tau
+
+end WBisim
+
+end Sme.ITree
+
